code/nist-pcurves/Hacl.Impl.PCurves.Compression.fsti
@@ -1,0 +1,46 @@
+module Hacl.Impl.PCurves.Compression
+
+open FStar.Mul
+open FStar.HyperStack.All
+open FStar.HyperStack
+module ST = FStar.HyperStack.ST
+
+open Lib.IntTypes
+open Lib.Buffer
+
+module S = Spec.PCurves
+
+#set-options "--z3rlimit 30 --fuel 0 --ifuel 0"
+
+inline_for_extraction noextract
+val uncompressed_to_raw: {| cp:S.curve_params |} -> pk:lbuffer uint8 (1ul +. 2ul *. size cp.bytes) ->
+                         pk_raw:lbuffer uint8 (2ul *. size cp.bytes) -> Stack bool
+  (requires fun h -> live h pk /\ live h pk_raw /\ disjoint pk pk_raw)
+  (ensures fun h0 b h1 -> modifies (loc pk_raw) h0 h1 /\
+    (b <==> Some? (S.pk_uncompressed_to_raw (as_seq h0 pk))) /\
+    (b ==> (as_seq h1 pk_raw == Some?.v (S.pk_uncompressed_to_raw (as_seq h0 pk)))))
+
+
+inline_for_extraction noextract
+val compressed_to_raw: {| cp:S.curve_params |} -> pk:lbuffer uint8 (1ul +. size cp.bytes) ->
+                       pk_raw:lbuffer uint8 (2ul *. size cp.bytes) -> Stack bool
+  (requires fun h -> live h pk /\ live h pk_raw /\ disjoint pk pk_raw)
+  (ensures  fun h0 b h1 -> modifies (loc pk_raw) h0 h1 /\
+    (b <==> Some? (S.pk_compressed_to_raw (as_seq h0 pk))) /\
+    (b ==> (as_seq h1 pk_raw == Some?.v (S.pk_compressed_to_raw (as_seq h0 pk)))))
+
+
+inline_for_extraction noextract
+val raw_to_uncompressed: {| cp:S.curve_params |} -> pk_raw:lbuffer uint8 (2ul *. size cp.bytes) ->
+                         pk:lbuffer uint8 (1ul +. 2ul *. size cp.bytes) -> Stack unit
+  (requires fun h -> live h pk /\ live h pk_raw /\ disjoint pk pk_raw)
+  (ensures fun h0 _ h1 -> modifies (loc pk) h0 h1 /\
+    as_seq h1 pk == S.pk_uncompressed_from_raw (as_seq h0 pk_raw))
+
+
+inline_for_extraction noextract
+val raw_to_compressed: {| cp:S.curve_params |} -> pk_raw:lbuffer uint8 (2ul *. size cp.bytes) ->
+                       pk:lbuffer uint8 (1ul +. size cp.bytes) -> Stack unit
+  (requires fun h -> live h pk /\ live h pk_raw /\ disjoint pk pk_raw)
+  (ensures  fun h0 _ h1 -> modifies (loc pk) h0 h1 /\
+    as_seq h1 pk == S.pk_compressed_from_raw (as_seq h0 pk_raw))
