code/nist-pcurves/Hacl.Impl.PCurves.Group.fst
@@ -1,0 +1,70 @@
+module Hacl.Impl.PCurves.Group
+
+open FStar.HyperStack
+open FStar.HyperStack.ST
+open FStar.Mul
+
+open Lib.IntTypes
+open Lib.Buffer
+
+module ST = FStar.HyperStack.ST
+module LSeq = Lib.Sequence
+
+module BE = Hacl.Impl.Exponentiation.Definitions
+
+module S = Spec.PCurves
+module SL = Spec.PCurves.Lemmas
+
+open Hacl.Impl.PCurves.Point
+
+#set-options "--z3rlimit 50 --fuel 0 --ifuel 0"
+
+unfold
+let linv_ctx (a:LSeq.lseq uint64 0) : Type0 = True
+
+unfold
+let refl {| cp:S.curve_params |} (p:LSeq.lseq uint64 (3*v cp.bn_limbs){point_inv_seq p}) : GTot S.aff_point =
+  S.to_aff_point (from_mont_point (as_point_nat_seq p))
+
+inline_for_extraction noextract
+let mk_to_pcurve_comm_monoid {| cp:S.curve_params |} : BE.to_comm_monoid U64 (3ul *. cp.bn_limbs) 0ul = {
+  BE.a_spec = S.aff_point;
+  BE.comm_monoid = S.mk_pcurve_comm_monoid;
+  BE.linv_ctx = linv_ctx;
+  BE.linv = point_inv_seq;
+  BE.refl = refl;
+}
+
+
+inline_for_extraction noextract
+val point_add {| cp:S.curve_params |} : BE.lmul_st U64 (3ul *. cp.bn_limbs) 0ul mk_to_pcurve_comm_monoid
+let point_add ctx x y xy =
+  let h0 = ST.get () in
+  SL.to_aff_point_add_lemma
+    (from_mont_point (as_point_nat h0 x)) (from_mont_point (as_point_nat h0 y));
+  Hacl.Impl.PCurves.PointAdd.point_add xy x y
+
+
+inline_for_extraction noextract
+val point_double {| cp:S.curve_params |} : BE.lsqr_st U64 (3ul *. cp.bn_limbs) 0ul mk_to_pcurve_comm_monoid
+let point_double ctx x xx =
+  let h0 = ST.get () in
+  SL.to_aff_point_double_lemma (from_mont_point (as_point_nat h0 x));
+  Hacl.Impl.PCurves.PointDouble.point_double xx x
+
+
+inline_for_extraction noextract
+val point_zero {| cp:S.curve_params |} : BE.lone_st U64 (3ul *. cp.bn_limbs) 0ul mk_to_pcurve_comm_monoid
+let point_zero {| cp:S.curve_params |} ctx one =
+  let h0 = ST.get () in
+  SL.to_aff_point_at_infinity_lemma #cp;
+  make_point_at_inf one
+
+
+inline_for_extraction noextract
+let mk_pcurve_concrete_ops {| cp:S.curve_params |} : BE.concrete_ops U64 (3ul *. cp.bn_limbs) 0ul = {
+  BE.to = mk_to_pcurve_comm_monoid;
+  BE.lone = point_zero;
+  BE.lmul = point_add;
+  BE.lsqr = point_double;
+}
