code/nist-pcurves/Hacl.Impl.PCurves.Point.fsti
@@ -1,0 +1,274 @@
+module Hacl.Impl.PCurves.Point
+
+open FStar.Mul
+open FStar.HyperStack.All
+open FStar.HyperStack
+
+open Lib.IntTypes
+open Lib.Buffer
+
+open Hacl.Impl.PCurves.Bignum
+
+module S = Spec.PCurves
+module SM = Hacl.Spec.PCurves.Montgomery
+module BD = Hacl.Spec.Bignum.Definitions
+module LSeq = Lib.Sequence
+
+#set-options "--z3rlimit 30 --fuel 0 --ifuel 0"
+
+let from_mont_point {| S.curve_params |} (a:tuple3 nat nat nat) : S.proj_point =
+  let x, y, z = a in SM.from_mont x, SM.from_mont y, SM.from_mont z
+
+
+///  Affine coordinates
+
+inline_for_extraction noextract
+let aff_point_seq {| cp:S.curve_params |} = LSeq.lseq uint64 (2 * v cp.bn_limbs)
+
+let as_aff_point_nat_seq {| cp:S.curve_params |} (p:aff_point_seq) =
+  BD.bn_v (LSeq.sub p 0 (v cp.bn_limbs)),
+  BD.bn_v (LSeq.sub p (v cp.bn_limbs) (v cp.bn_limbs))
+
+let aff_point_inv_seq {| S.curve_params |} (p:aff_point_seq) =
+  let x, y = as_aff_point_nat_seq p in
+  x < S.prime /\ y < S.prime
+
+
+inline_for_extraction noextract
+let aff_point {| cp:S.curve_params |} = lbuffer uint64 (2ul *. S.bn_limbs)
+
+noextract
+let as_aff_point_nat {| cp:S.curve_params |} (h:mem) (p:aff_point) =
+  as_aff_point_nat_seq (as_seq h p)
+
+noextract
+let aff_point_inv {| S.curve_params |} (h:mem) (p:aff_point) =
+  aff_point_inv_seq (as_seq h p)
+
+noextract
+let as_aff_point_nat_inv {| cp:S.curve_params |} (h:mem) (p:aff_point{aff_point_inv h p}) : GTot S.aff_point  =
+  let (x,y)= as_aff_point_nat h p in (x,y)
+
+noextract
+let aff_point_x_as_nat {| cp:S.curve_params |} (h:mem) (p:aff_point) : GTot nat =
+  as_nat h (gsub p 0ul cp.bn_limbs)
+
+noextract
+let aff_point_y_as_nat {| cp:S.curve_params |} (h:mem) (p:aff_point) : GTot nat =
+  as_nat h (gsub p cp.bn_limbs cp.bn_limbs)
+
+inline_for_extraction noextract
+let aff_getx {| cp:S.curve_params |} (p:aff_point) : Stack felem
+  (requires fun h -> live h p)
+  (ensures fun h0 f h1 -> f == gsub p 0ul cp.bn_limbs /\ h0 == h1)
+  = sub p 0ul cp.bn_limbs
+
+inline_for_extraction noextract
+let aff_gety {| cp:S.curve_params |} (p:aff_point) : Stack felem
+  (requires fun h -> live h p)
+  (ensures fun h0 f h1 -> f == gsub p cp.bn_limbs cp.bn_limbs /\ h0 == h1)
+  = sub p cp.bn_limbs cp.bn_limbs
+
+
+///  Projective coordinates
+
+inline_for_extraction noextract
+let point_seq {| cp:S.curve_params |} = LSeq.lseq uint64 (3 * v cp.bn_limbs)
+
+noextract
+let as_point_nat_seq {| cp:S.curve_params |} (p:point_seq) =
+  BD.bn_v (LSeq.sub p 0 (v cp.bn_limbs)),
+  BD.bn_v (LSeq.sub p (v cp.bn_limbs) (v cp.bn_limbs)),
+  BD.bn_v (LSeq.sub p (2 * v cp.bn_limbs) (v cp.bn_limbs))
+
+noextract
+let point_inv_seq {| S.curve_params |} (p:point_seq) =
+  let x, y, z = as_point_nat_seq p in
+  x < S.prime /\ y < S.prime /\ z < S.prime
+
+
+inline_for_extraction noextract
+let point {| cp:S.curve_params |} = lbuffer uint64 (3ul *. cp.bn_limbs)
+
+noextract
+let as_point_nat {| cp:S.curve_params |} (h:mem) (p:point) =
+  as_point_nat_seq (as_seq h p)
+
+noextract
+let point_inv {| S.curve_params |} (h:mem) (p:point) =
+  point_inv_seq (as_seq h p)
+
+noextract
+let as_point_nat_inv {| cp:S.curve_params |} (h:mem) (p:point{point_inv h p}) : GTot S.proj_point =
+  let (x,y,z) = as_point_nat h p  in (x,y,z)
+
+noextract
+let point_x_as_nat {| cp:S.curve_params |} (h:mem) (p:point) : GTot nat =
+  as_nat h (gsub p 0ul cp.bn_limbs)
+
+noextract
+let point_y_as_nat {| cp:S.curve_params |} (h:mem) (e:point) : GTot nat =
+  as_nat h (gsub e cp.bn_limbs cp.bn_limbs)
+
+noextract
+let point_z_as_nat {| cp:S.curve_params |} (h:mem) (e:point) : GTot nat =
+  as_nat h (gsub e (2ul *. cp.bn_limbs) (cp.bn_limbs))
+
+
+inline_for_extraction noextract
+let getx {| cp:S.curve_params |} (p:point) : Stack felem
+  (requires fun h -> live h p)
+  (ensures fun h0 f h1 -> f == gsub p 0ul cp.bn_limbs /\ h0 == h1)
+  = sub p 0ul cp.bn_limbs
+
+inline_for_extraction noextract
+let gety {| cp:S.curve_params |} (p:point) : Stack felem
+  (requires fun h -> live h p)
+  (ensures fun h0 f h1 -> f == gsub p cp.bn_limbs cp.bn_limbs /\ h0 == h1)
+  = sub p cp.bn_limbs cp.bn_limbs
+
+#push-options "--z3rlimit 700"
+inline_for_extraction noextract
+let getz {| cp:S.curve_params |} (p:point) : Stack felem
+  (requires fun h -> live h p)
+  (ensures fun h0 f h1 -> f == gsub p (2ul *. cp.bn_limbs) (cp.bn_limbs) /\ h0 == h1)
+  = assert (v (2ul *. cp.bn_limbs) == 2 * v cp.bn_limbs);
+    sub p (2ul *. cp.bn_limbs) (cp.bn_limbs)
+#pop-options
+
+///  Create a point
+
+inline_for_extraction noextract
+val create_aff_point: {| cp:S.curve_params |} -> StackInline aff_point
+  (requires fun h -> True)
+  (ensures  fun h0 f h1 ->
+    stack_allocated f h0 h1 (LSeq.create (2 * v cp.bn_limbs) (u64 0)))
+
+
+inline_for_extraction noextract
+val create_point: {| cp:S.curve_params |} -> StackInline point
+  (requires fun h -> True)
+  (ensures  fun h0 f h1 ->
+    stack_allocated f h0 h1 (LSeq.create (3 * v cp.bn_limbs) (u64 0)))
+
+
+val make_base_point: {| S.curve_params |} -> p:point -> Stack unit
+  (requires fun h -> live h p)
+  (ensures fun h0 _ h1 -> modifies (loc p) h0 h1 /\
+    point_inv h1 p /\ from_mont_point (as_point_nat h1 p) == S.base_point)
+
+
+val make_point_at_inf: {| S.curve_params |} -> p:point -> Stack unit
+  (requires fun h -> live h p)
+  (ensures fun h0 _ h1 -> modifies (loc p) h0 h1 /\
+    point_inv h1 p /\ from_mont_point (as_point_nat h1 p) == S.point_at_inf)
+
+
+///  Check if a point is a point-at-infinity
+
+val is_point_at_inf: {| S.curve_params |} -> p:point -> Stack uint64
+  (requires fun h -> live h p /\ point_inv h p)
+  (ensures fun h0 r h1 -> modifies0 h0 h1 /\
+    (let pM = from_mont_point (as_point_nat h0 p) in
+    (if S.is_point_at_inf pM then v r = ones_v U64 else v r = 0) /\
+    (if S.is_point_at_inf (as_point_nat_inv h0 p) then v r = ones_v U64 else v r = 0)))
+
+
+val is_point_at_inf_vartime: {| S.curve_params |} -> p:point -> Stack bool
+  (requires fun h -> live h p /\ point_inv h p)
+  (ensures  fun h0 r h1 -> modifies0 h0 h1 /\
+    r == S.is_point_at_inf (as_point_nat_inv h0 p) /\
+    r == S.is_point_at_inf (from_mont_point (as_point_nat h0 p)))
+
+
+///  Create a copy of a point
+
+inline_for_extraction noextract
+val copy_point: {| S.curve_params |} -> res:point -> p:point -> Stack unit
+  (requires fun h -> live h p /\ live h res /\ disjoint p res)
+  (ensures fun h0 _ h1 -> modifies (loc res) h0 h1 /\
+    as_seq h1 res == as_seq h0 p)
+
+
+///  Point conversion between Projective and Affine coordinates representations
+
+// to_aff_point = S.to_aff_point + from_mont
+val to_aff_point: {| S.curve_params |} -> res:aff_point -> p:point -> Stack unit
+  (requires fun h ->
+    live h p /\ live h res /\ eq_or_disjoint p res /\
+    point_inv h p)
+  (ensures fun h0 _ h1 -> modifies (loc res) h0 h1 /\
+    aff_point_inv h1 res /\
+    as_aff_point_nat_inv h1 res == S.to_aff_point (from_mont_point (as_point_nat h0 p)))
+
+
+// to_aff_point = S.to_aff_point + from_mont
+val to_aff_point_x: {| S.curve_params |} -> res:felem -> p:point -> Stack unit
+  (requires fun h ->
+    live h p /\ live h res /\ eq_or_disjoint p res /\
+    point_inv h p)
+  (ensures fun h0 _ h1 -> modifies (loc res) h0 h1 /\
+    as_nat h1 res == fst (S.to_aff_point (from_mont_point (as_point_nat h0 p))))
+
+
+// to_proj_point = S.to_proj_point + to_mont
+val to_proj_point: {| S.curve_params |} -> res:point -> p:aff_point -> Stack unit
+  (requires fun h ->
+    live h p /\ live h res /\ disjoint p res /\
+    aff_point_inv h p)
+  (ensures  fun h0 _ h1 -> modifies (loc res) h0 h1 /\
+    point_inv h1 res /\
+    from_mont_point (as_point_nat h1 res) == S.to_proj_point (as_aff_point_nat_inv h0 p))
+
+
+///  Check if a point is on the curve
+
+val is_on_curve_vartime: {| S.curve_params |} -> p:aff_point -> Stack bool
+  (requires fun h -> live h p /\ aff_point_inv h p)
+  (ensures fun h0 r h1 -> modifies0 h0 h1 /\
+    r == S.is_on_curve (as_aff_point_nat_inv h0 p))
+
+
+///  Point load and store functions
+
+val aff_point_store: {| cp:S.curve_params |} -> res:lbuffer uint8 (2ul *. size cp.bytes) -> p:aff_point -> Stack unit
+  (requires fun h ->
+    live h res /\ live h p /\ disjoint res p /\
+    aff_point_inv h p)
+  (ensures  fun h0 _ h1 -> modifies (loc res) h0 h1 /\
+    as_seq h1 res == S.aff_point_store (as_aff_point_nat_inv h0 p))
+
+
+val point_store: {| cp:S.curve_params |} -> res:lbuffer uint8 (2ul *. size cp.bytes) -> p:point -> Stack unit
+  (requires fun h ->
+    live h res /\ live h p /\ disjoint res p /\
+    point_inv h p)
+  (ensures  fun h0 _ h1 -> modifies (loc res) h0 h1 /\
+    as_seq h1 res == S.point_store (from_mont_point (as_point_nat h0 p)))
+
+
+val aff_point_load_vartime: {| cp:S.curve_params |} -> res:aff_point -> b:lbuffer uint8 (2ul *. size cp.bytes) -> Stack bool
+  (requires fun h ->
+    live h res /\ live h b /\ disjoint res b)
+  (ensures  fun h0 r h1 -> modifies (loc res) h0 h1 /\
+    (let ps = S.aff_point_load (as_seq h0 b) in
+    (r <==> Some? ps) /\ (r ==> (aff_point_inv h1 res /\ as_aff_point_nat_inv h1 res == Some?.v ps))))
+
+
+val load_point_vartime: {| cp:S.curve_params |} -> res:point -> b:lbuffer uint8 (2ul *. size cp.bytes) -> Stack bool
+  (requires fun h ->
+    live h res /\ live h b /\ disjoint res b)
+  (ensures  fun h0 r h1 -> modifies (loc res) h0 h1 /\
+    (let ps = S.load_point (as_seq h0 b) in
+    (r <==> Some? ps) /\ (r ==> (point_inv h1 res /\
+      from_mont_point (as_point_nat h1 res) == Some?.v ps))))
+
+
+val aff_point_decompress_vartime {| S.curve_params |} (x y:felem) (s:lbuffer uint8 (1ul +. (size S.bytes))) : Stack bool
+  (requires fun h ->
+    live h x /\ live h y /\ live h s /\
+    disjoint x y /\ disjoint x s /\ disjoint y s)
+  (ensures fun h0 b h1 -> modifies (loc x |+| loc y) h0 h1 /\
+    (b <==> Some? (S.aff_point_decompress (as_seq h0 s))) /\
+    (b ==> (let (xa, ya) = Some?.v (S.aff_point_decompress (as_seq h0 s)) in
+    as_nat h1 x < S.prime /\ as_nat h1 y < S.prime /\ as_nat h1 x == xa /\ as_nat h1 y == ya)))
