code/nist-pcurves/Hacl.Impl.PCurves.PointDouble.fsti
@@ -1,0 +1,23 @@
+module Hacl.Impl.PCurves.PointDouble
+
+open FStar.HyperStack.All
+open FStar.HyperStack
+module ST = FStar.HyperStack.ST
+
+open Lib.IntTypes
+open Lib.Buffer
+
+open Hacl.Impl.PCurves.Point
+
+module S = Spec.PCurves
+
+#set-options "--z3rlimit 30 --fuel 0 --ifuel 0"
+
+val point_double: {| cp:S.curve_params |} -> res:point -> p:point -> Stack unit
+  (requires fun h ->
+    live h p /\ live h res /\ eq_or_disjoint p res /\
+    point_inv h p)
+  (ensures fun h0 _ h1 -> modifies (loc res)  h0 h1 /\
+    point_inv h1 res /\
+    from_mont_point (as_point_nat h1 res) ==
+      S.point_double (from_mont_point (as_point_nat h0 p)))
