code/nist-pcurves/Hacl.Impl.PCurves.PointMul.fsti
@@ -1,0 +1,53 @@
+module Hacl.Impl.PCurves.PointMul
+
+open FStar.Mul
+open FStar.HyperStack.All
+open FStar.HyperStack
+module ST = FStar.HyperStack.ST
+
+open Lib.IntTypes
+open Lib.Buffer
+
+open Hacl.Impl.PCurves.Bignum
+open Hacl.Impl.PCurves.Point
+
+module S = Spec.PCurves
+
+include Hacl.Impl.PCurves.Group
+include Hacl.PCurves.PrecompTable
+
+
+#set-options "--z3rlimit 30 --fuel 0 --ifuel 0"
+
+val point_mul: {| cp:S.curve_params |} -> {| pt:precomp_tables |} -> res:point -> scalar:felem -> p:point -> Stack unit
+  (requires fun h ->
+    live h p /\ live h res /\ live h scalar /\
+    disjoint p res /\ disjoint scalar res /\ disjoint p scalar /\
+    point_inv h p /\ as_nat h scalar < S.order)
+  (ensures fun h0 _ h1 -> modifies (loc res) h0 h1 /\
+    point_inv h1 res /\
+    S.to_aff_point (from_mont_point (as_point_nat h1 res)) ==
+    S.to_aff_point (S.point_mul (as_nat h0 scalar) (from_mont_point (as_point_nat h0 p))))
+
+
+val point_mul_g: {| cp:S.curve_params |} -> {| pt:precomp_tables |} -> res:point -> scalar:felem -> Stack unit
+  (requires fun h ->
+    live h res /\ live h scalar /\ disjoint res scalar /\
+    as_nat h scalar < S.order)
+  (ensures fun h0 _ h1 -> modifies (loc res) h0 h1 /\
+    point_inv h1 res /\
+    S.to_aff_point (from_mont_point (as_point_nat h1 res)) ==
+    S.to_aff_point (S.point_mul_g (as_nat h0 scalar)))
+
+
+val point_mul_double_g: {| cp:S.curve_params |} -> {| pt:precomp_tables |} -> res:point -> scalar1:felem -> scalar2:felem -> p:point -> Stack unit
+  (requires fun h ->
+    live h res /\ live h scalar1 /\ live h scalar2 /\ live h p /\
+    disjoint res scalar1 /\ disjoint res scalar2 /\ disjoint res p /\
+    disjoint p scalar1 /\ disjoint p scalar2 /\
+    point_inv h p /\ as_nat h scalar1 < S.order /\ as_nat h scalar2 < S.order)
+  (ensures  fun h0 _ h1 -> modifies (loc res) h0 h1 /\
+    point_inv h1 res /\
+    S.to_aff_point (from_mont_point (as_point_nat h1 res)) ==
+    S.to_aff_point (S.point_mul_double_g (as_nat h0 scalar1) (as_nat h0 scalar2)
+      (from_mont_point (as_point_nat h0 p))))
