code/nist-pcurves/Hacl.Impl.PCurves.Qinv.fsti
@@ -1,0 +1,24 @@
+module Hacl.Impl.PCurves.Qinv
+
+open FStar.Mul
+open FStar.HyperStack.All
+open FStar.HyperStack
+module ST = FStar.HyperStack.ST
+
+open Lib.IntTypes
+open Lib.Buffer
+
+open Hacl.Impl.PCurves.Bignum
+open Hacl.Impl.PCurves.Scalar
+
+module S = Spec.PCurves
+
+#set-options "--z3rlimit 30 --fuel 0 --ifuel 0"
+
+val qinv: {| cp:S.curve_params |} -> res:felem -> a:felem -> Stack unit
+  (requires fun h ->
+    live h a /\ live h res /\ eq_or_disjoint a res /\
+    as_nat h a < S.order)
+  (ensures fun h0 _ h1 -> modifies (loc res) h0 h1 /\
+    as_nat h1 res < S.order /\
+    qmont_as_nat h1 res == S.qinv (qmont_as_nat h0 a))
