code/nist-pcurves/Hacl.PCurves.PrecompTable.fst
@@ -1,0 +1,101 @@
+module Hacl.PCurves.PrecompTable
+
+open FStar.HyperStack
+open FStar.HyperStack.ST
+open FStar.Mul
+
+open Lib.IntTypes
+open Lib.Buffer
+
+module ST = FStar.HyperStack.ST
+module LSeq = Lib.Sequence
+
+module LE = Lib.Exponentiation
+module SE = Spec.Exponentiation
+module SPT = Hacl.Spec.PrecompBaseTable
+module SPT256 = Hacl.Spec.PrecompBaseTable256
+module SPTK = Hacl.Spec.PCurves.PrecompTable
+
+module S = Spec.PCurves
+module SL = Spec.PCurves.Lemmas
+
+open Hacl.Impl.PCurves.Point
+include Hacl.Impl.PCurves.Group
+
+#set-options "--z3rlimit 50 --fuel 0 --ifuel 0"
+
+let proj_point_to_list {| cp:S.curve_params |} p =
+  SPTK.proj_point_to_list_lemma p;
+  SPTK.proj_point_to_list p
+
+let lemma_refl {| cp:S.curve_params |} x =
+  SPTK.proj_point_to_list_lemma x
+
+//-----------------
+
+inline_for_extraction noextract
+let proj_g_pow2_64_list {| S.curve_params |} {| precomp_g_points |} : SPTK.point_list =
+  normalize_term (SPTK.proj_point_to_list proj_g_pow2_64)
+
+inline_for_extraction noextract
+let proj_g_pow2_128_list {| S.curve_params |} {| precomp_g_points |} : SPTK.point_list =
+  normalize_term (SPTK.proj_point_to_list proj_g_pow2_128)
+
+inline_for_extraction noextract
+let proj_g_pow2_192_list {| S.curve_params |} {| precomp_g_points |} : SPTK.point_list =
+  normalize_term (SPTK.proj_point_to_list proj_g_pow2_192)
+
+let proj_g_pow2_64_lseq {| cp:S.curve_params |} {| p:precomp_g_points |} : LSeq.lseq uint64 (3 * v S.bn_limbs) =
+  normalize_term_spec (SPTK.proj_point_to_list proj_g_pow2_64);
+  Seq.seq_of_list (proj_g_pow2_64_list #cp #p)
+
+let proj_g_pow2_128_lseq {| cp:S.curve_params |} {| p:precomp_g_points |} : LSeq.lseq uint64 (3 * v cp.bn_limbs)  =
+  normalize_term_spec (SPTK.proj_point_to_list proj_g_pow2_128);
+  Seq.seq_of_list proj_g_pow2_128_list
+
+let proj_g_pow2_192_lseq {| cp:S.curve_params |} {| p:precomp_g_points |} : LSeq.lseq uint64 (3 * v cp.bn_limbs) =
+  normalize_term_spec (SPTK.proj_point_to_list proj_g_pow2_192);
+  Seq.seq_of_list proj_g_pow2_192_list
+
+let proj_g_pow2_64_lemma {| cp:S.curve_params |} {| p:precomp_g_points |} () =
+  p.lemma_proj_g_pow2_64_eval ();
+  SPT256.a_pow2_64_lemma S.mk_pcurve_concrete_ops S.base_point
+
+let proj_g_pow2_128_lemma {| cp:S.curve_params |} {| p:precomp_g_points |} () =
+  p.lemma_proj_g_pow2_128_eval ();
+  p.lemma_proj_g_pow2_64_eval ();
+  SPT256.a_pow2_128_lemma S.mk_pcurve_concrete_ops S.base_point
+
+let proj_g_pow2_192_lemma {| cp:S.curve_params |} {| p:precomp_g_points |} () =
+  p.lemma_proj_g_pow2_192_eval ();
+  p.lemma_proj_g_pow2_128_eval ();
+  p.lemma_proj_g_pow2_64_eval ();
+  SPT256.a_pow2_192_lemma S.mk_pcurve_concrete_ops S.base_point
+
+let proj_g_pow2_64_lseq_lemma {| cp:S.curve_params |} {| p:precomp_g_points |} () =
+  normalize_term_spec (SPTK.proj_point_to_list p.proj_g_pow2_64);
+  proj_g_pow2_64_lemma ();
+  SPTK.proj_point_to_list_lemma p.proj_g_pow2_64
+
+let proj_g_pow2_128_lseq_lemma {| cp:S.curve_params |} {| p:precomp_g_points |} () =
+  normalize_term_spec (SPTK.proj_point_to_list proj_g_pow2_128);
+  proj_g_pow2_128_lemma ();
+  SPTK.proj_point_to_list_lemma proj_g_pow2_128
+
+
+let proj_g_pow2_192_lseq_lemma {| cp:S.curve_params |} {| p:precomp_g_points |} () =
+  normalize_term_spec (SPTK.proj_point_to_list proj_g_pow2_192);
+  proj_g_pow2_192_lemma ();
+  SPTK.proj_point_to_list_lemma proj_g_pow2_192
+
+#push-options "--fuel 1"
+let mk_proj_g_pow2_64 {| cp:S.curve_params |} {| p:precomp_g_points |} () =
+  createL proj_g_pow2_64_list
+
+let mk_proj_g_pow2_128 {| cp:S.curve_params |} {| p:precomp_g_points |} () =
+  createL proj_g_pow2_128_list
+
+let mk_proj_g_pow2_192 {| cp:S.curve_params |} {| p:precomp_g_points |} () =
+  createL proj_g_pow2_192_list
+#pop-options
+
