code/nist-pcurves/Hacl.Spec.PCurves.PrecompTable.fst
@@ -1,0 +1,123 @@
+module Hacl.Spec.PCurves.PrecompTable
+
+open FStar.Mul
+open Lib.IntTypes
+open Lib.Sequence
+
+open Hacl.Impl.PCurves.Point
+
+module S = Spec.PCurves
+module SM = Hacl.Spec.PCurves.Montgomery
+module BD = Hacl.Spec.Bignum.Definitions
+module FL = FStar.List.Tot
+module SPT = Hacl.Spec.PrecompBaseTable
+
+#set-options "--z3rlimit 50 --fuel 0 --ifuel 0"
+
+let create4_lseq (x0 x1 x2 x3:uint64) : lseq uint64 4 =
+  let l = [x0; x1; x2; x3] in
+  assert_norm (FL.length l = 4);
+  Seq.seq_of_list l
+
+
+val create4_lemma (x0 x1 x2 x3:uint64) :
+  Lemma (let s = create4_lseq x0 x1 x2 x3 in
+    s.[0] == x0 /\ s.[1] == x1 /\ s.[2] == x2 /\ s.[3] == x3)
+let create4_lemma x0 x1 x2 x3 =
+  Seq.elim_of_list [x0; x1; x2; x3]
+
+//-----------------------------------
+
+noextract
+let list_as_felem {| cp:S.curve_params |} (f:felem_list) : lseq uint64 (v cp.bn_limbs) =
+  Seq.seq_of_list f <: lseq uint64 (v cp.bn_limbs)
+
+
+val felem_to_list_lemma_eval: {| cp:S.curve_params |} -> x:S.felem ->
+  Lemma (BD.bn_v (list_as_felem (felem_to_list x)) == x)
+
+let felem_to_list_lemma_eval {| cp:S.curve_params |} x =
+  if cp.bn_limbs = 4ul then (
+    assume (cp.bits == 256);
+    let x0 = x % pow2 64 in
+    let x1 = x / pow2 64 % pow2 64 in
+    let x2 = x / pow2 128 % pow2 64 in
+    let x3 = x / pow2 192 % pow2 64 in
+    let bn_x = list_as_felem (felem_to_list x) in
+    create4_lemma (u64 x0) (u64 x1) (u64 x2) (u64 x3);
+      assert (v bn_x.[0] == x0 /\ v bn_x.[1] == x1 /\ v bn_x.[2] == x2 /\ v bn_x.[3] == x3);
+    Hacl.Impl.PCurves.Bignum.bn_v_is_as_nat4 bn_x;
+      assert (BD.bn_v bn_x = x0 + x1 * pow2 64 + x2 * pow2 128 + x3 * pow2 192);
+    Hacl.Spec.PrecompBaseTable256.lemma_decompose_nat256_as_four_u64 x)
+  else admit()
+
+//--------------------------------------------
+
+val proj_point_to_list_sub {| cp:S.curve_params |} : p:S.proj_point -> Lemma
+ (let (px, py, pz) = p in
+  let pxM = SM.to_mont px in
+  let pyM = SM.to_mont py in
+  let pzM = SM.to_mont pz in
+  let px_list = felem_to_list pxM in
+  let py_list = felem_to_list pyM in
+  let pz_list = felem_to_list pzM in
+  let p_list = FL.(px_list @ py_list @ pz_list) in
+
+  let p_lseq = Seq.seq_of_list p_list <: lseq uint64 (3 * v cp.bn_limbs) in
+  let px_lseq = Seq.seq_of_list px_list <: lseq uint64 (v cp.bn_limbs) in
+  let py_lseq = Seq.seq_of_list py_list <: lseq uint64 (v cp.bn_limbs) in
+  let pz_lseq = Seq.seq_of_list pz_list <: lseq uint64 (v cp.bn_limbs) in
+  sub p_lseq 0 (v cp.bn_limbs) == px_lseq /\
+  sub p_lseq (v cp.bn_limbs) (v cp.bn_limbs) == py_lseq /\
+  sub p_lseq (2 * v cp.bn_limbs) (v cp.bn_limbs) == pz_lseq)
+
+let proj_point_to_list_sub {| cp:S.curve_params |} p =
+  let (px, py, pz) = p in
+  let pxM = SM.to_mont px in
+  let pyM = SM.to_mont py in
+  let pzM = SM.to_mont pz in
+  let px_list = felem_to_list pxM in
+  let py_list = felem_to_list pyM in
+  let pz_list = felem_to_list pzM in
+
+  FL.append_assoc px_list py_list pz_list;
+  SPT.seq_of_list_append_lemma px_list py_list;
+  SPT.seq_of_list_append_lemma FL.(px_list @ py_list) pz_list
+
+
+val proj_point_to_list_fits {| cp:S.curve_params |} : p:S.proj_point ->
+  Lemma (point_inv_list (proj_point_to_list p))
+
+let proj_point_to_list_fits {| cp:S.curve_params |} p =
+  let (px, py, pz) = p in
+  let pxM = SM.to_mont px in
+  let pyM = SM.to_mont py in
+  let pzM = SM.to_mont pz in
+
+  proj_point_to_list_sub p;
+  felem_to_list_lemma_eval pxM;
+  felem_to_list_lemma_eval pyM;
+  felem_to_list_lemma_eval pzM
+
+
+val proj_point_to_list_eval: {| cp:S.curve_params |} -> p:S.proj_point ->
+  Lemma (point_eval_list (proj_point_to_list p) == p) 
+
+let proj_point_to_list_eval p =
+  let (px, py, pz) = p in
+  let pxM = SM.to_mont px in
+  let pyM = SM.to_mont py in
+  let pzM = SM.to_mont pz in
+
+  proj_point_to_list_sub p;
+  felem_to_list_lemma_eval pxM;
+  felem_to_list_lemma_eval pyM;
+  felem_to_list_lemma_eval pzM;
+  SM.lemma_to_from_mont_id px;
+  SM.lemma_to_from_mont_id py;
+  SM.lemma_to_from_mont_id pz
+
+
+let proj_point_to_list_lemma p =
+  proj_point_to_list_fits p;
+  proj_point_to_list_eval p
